Simplified away the context's reference (shared one seems enough)

state/SimpleState.fst
@@ -2,10 +2,8 @@ module SimpleState
 
 open FStar.Ref
 
-assume val trp : Type // Type of the reference of the program
-assume val trc : Type // Type of the reference of the context
-                      // <- unclear if this reference really needed; shared good enough?
-assume val trs : Type // Type of the reference that's shared
+assume val trp : Type // Type of the reference of the program (not shared)
+assume val trs : Type // Type of the reference *shared* between program and context
                       // <- for now let's assume this is not refined
 assume val t1 : Type
 assume val t2 : Type
@@ -13,84 +11,74 @@ assume val t2 : Type
 // Simple target types
 
 // Target type of whole program
-let t_tw : Type = ref trp -> ref trc -> ref trs -> St int
+let t_tw : Type = ref trp -> ref trs -> St int
 
 // Target type of context
-let t_tc : Type = ref trc -> ref trs -> t1 -> St t2
+let t_tc : Type = ref trs -> t1 -> St t2
 
 // Target type of program -- has initial control, calls context
 let t_tp : Type = ref trp -> ref trs -> (t1 -> St t2) -> St int
 
 let t_link (t_p:t_tp) (t_c:t_tc) : t_tw =
-  fun (rp:ref trp) (rc:ref trc) (rs:ref trs) ->
-    t_p rp rs (t_c rc rs)
+  fun (rp:ref trp) (rs:ref trs) ->
+    t_p rp rs (t_c rs)
 
 // Refined source types
 
 // This separation invariant used for both program and context
-let sep (rp:ref trp) (rc:ref trc) (rs:ref trs) (h0:heap) : Type0 =
-  (* initial references are not aliasing:
-     (what hyper-heap regions could give us?) *)
-  addr_of rp <> addr_of rc /\
+let sep (rp:ref trp) (rs:ref trs) (h0:heap) : Type0 =
+  (* initial references are not aliasing: (what hyper-heap regions could give us?) *)
   addr_of rp <> addr_of rs /\
-  addr_of rc <> addr_of rs /\
-  (* initial references allocated: *)
-  h0 `contains` rp /\ h0 `contains` rc /\ h0 `contains` rs
-  (* + TODO (hard in general!?): rp is not reachable from rc and rs *)
+  (* initial references are allocated: *)
+  h0 `contains` rp /\ h0 `contains` rs
+  (* + TODO (hard in general!?): rp is not reachable from rs *)
 
-assume val post_prog : ref trp -> ref trc -> ref trs -> heap -> int -> heap -> Type0
-// user defined and proved statically about the partial program
+assume val post_prog : ref trp -> ref trs -> heap -> int -> heap -> Type0
+// <- user defined and proved statically about the partial program
 
-let s_tw : Type = rp:ref trp -> rc:ref trc -> rs:ref trs ->
-  ST int (requires (fun h0 -> sep rp rc rs h0))
-         (ensures (fun h0 res h1 -> post_prog rp rc rs h0 res h1))
+let s_tw : Type = rp:ref trp -> rs:ref trs ->
+  ST int (requires (fun h0 -> sep rp rs h0))
+         (ensures (fun h0 res h1 -> post_prog rp rs h0 res h1))
 
-assume val pre_ctx : ref trc -> ref trs -> t1 -> heap -> Type0
-// user defined and proved statically about the partial program (who calls context)
+assume val pre_ctx : ref trs -> t1 -> heap -> Type0
+// <- user defined and proved statically about the partial program (who calls context)
 
-assume val post_ctx : ref trc -> ref trs -> t1 -> heap -> t2 -> heap -> Type0
+assume val post_ctx : ref trs -> t1 -> heap -> t2 -> heap -> bool
 // dynamically enforced when the context returns control back to the program
+// (so for now going directly to bool)
 
-let s_tc (rp:ref trp) : Type = rc:ref trc -> rs:ref trs -> arg:t1 ->
-  ST t2 (requires (fun h0 -> sep rp rc rs h0 /\ pre_ctx rc rs arg h0))
-        (ensures (fun h0 res h1 -> sep rp rc rs h1 // <- necessarily preserved by context
-          /\ post_ctx rc rs arg h0 res h1 // <- dynamically enforced
+let s_tc (rp:ref trp) : Type = rs:ref trs -> arg:t1 ->
+  ST t2 (requires (fun h0 -> sep rp rs h0 /\ pre_ctx rs arg h0))
+        (ensures (fun h0 res h1 -> sep rp rs h1 // <- necessarily preserved by context
+          /\ post_ctx rs arg h0 res h1 // <- dynamically enforced
           /\ sel h0 rp == sel h1 rp)) // <- enforced by state separation
 
 // putting together the types + specs above
-let s_tp (rc:ref trc) : Type = rp:ref trp -> rs:ref trs ->
-  (arg:t1 -> ST t2 (requires (fun h0 -> sep rp rc rs h0 /\ pre_ctx rc rs arg h0))
-                   (ensures (fun h0 res h1 -> sep rp rc rs h1
-                     /\ post_ctx rc rs arg h0 res h1
+let s_tp : Type = rp:ref trp -> rs:ref trs ->
+  (arg:t1 -> ST t2 (requires (fun h0 -> sep rp rs h0 /\ pre_ctx rs arg h0))
+                   (ensures (fun h0 res h1 -> sep rp rs h1
+                     /\ post_ctx rs arg h0 res h1
                      /\ sel h0 rp == sel h1 rp))) ->
-  ST int (requires (fun h0 -> sep rp rc rs h0))
-         (ensures (fun h0 res h1 -> post_prog rp rc rs h0 res h1))
+  ST int (requires (fun h0 -> sep rp rs h0))
+         (ensures (fun h0 res h1 -> post_prog rp rs h0 res h1))
 
-// Problem: had to change order of arguments to use rp and rc
+// Problem: had to change order of arguments to use rp in context type
 //          (so this doesn't return a s_tw)
-let s_link (rp:ref trp) (rc:ref trc) (s_p:s_tp rc) (s_c:s_tc rp) (rs:ref trs) :
-  ST int (requires (fun h0 -> sep rp rc rs h0))
-         (ensures (fun h0 res h1 -> post_prog rp rc rs h0 res h1)) =
-  s_p rp rs (s_c rc rs)
+let s_link (s_p:s_tp) (rp:ref trp) (s_c:s_tc rp) (rs:ref trs) :
+  ST int (requires (fun h0 -> sep rp rs h0))
+         (ensures (fun h0 res h1 -> post_prog rp rs h0 res h1)) =
+  s_p rp rs (s_c rs)
 
 // Solution using erased references
 
 open FStar.Ghost
 
-let se_tc : Type = erp:erased (ref trp) -> rc:ref trc -> rs:ref trs -> arg:t1 ->
-  ST t2 (requires (fun h0 -> sep erp rc rs h0 /\ pre_ctx rc rs arg h0))
-        (ensures (fun h0 res h1 -> sep erp rc rs h1 // <- necessarily preserved by context
-          /\ post_ctx rc rs arg h0 res h1 // <- dynamically enforced
+let se_tc : Type = erp:erased (ref trp) -> rs:ref trs -> arg:t1 ->
+  ST t2 (requires (fun h0 -> sep erp rs h0 /\ pre_ctx rs arg h0))
+        (ensures (fun h0 res h1 -> sep erp rs h1 // <- necessarily preserved by context
+          /\ post_ctx rs arg h0 res h1 // <- dynamically enforced
           /\ sel h0 erp == sel h1 erp)) // <- enforced by state separation
 
-let se_tp : Type = rp:ref trp -> erc: erased (ref trc) -> rs:ref trs ->
-  (arg:t1 -> ST t2 (requires (fun h0 -> sep rp erc rs h0 /\ pre_ctx erc rs arg h0))
-                   (ensures (fun h0 res h1 -> sep rp erc rs h1
-                     /\ post_ctx erc rs arg h0 res h1
-                     /\ sel h0 rp == sel h1 rp))) ->
-  ST int (requires (fun h0 -> sep rp erc rs h0))
-         (ensures (fun h0 res h1 -> post_prog rp erc rs h0 res h1))
-
-let se_link (s_p:se_tp) (s_c:se_tc) : s_tw =
-  fun (rp:ref trp) (rc:ref trc) (rs:ref trs) ->
-    s_p rp rc rs (s_c rp rc rs)
+let se_link (s_p:s_tp) (s_c:se_tc) : s_tw =
+  fun (rp:ref trp) (rs:ref trs) ->
+    s_p rp rs (s_c rp rs)
